cnf.dfy
@@ -1,0 +1,25 @@
+include "sat.dfy"
+
+// Clause: l1 ∨ l2 ∨ ... ∨ ln
+// CNF: C1 ∧ C2 ∧ ... ∧ Cn
+
+function clause_is_tautology(c: Clause) : (out: bool)
+    ensures out ==> (
+        forall vs: map<Variable,bool> :: true ==> clause_eval(c, vs) == true
+    )
+{
+    exists l1,l2 :: l1 in c && l2 in c && l1.invert() == l2
+}
+
+ghost function cnf_equivalent(cnf: CNF, other: CNF) : (eq: bool)
+{
+    forall vs : map<Variable, bool> :: true ==>
+        cnf_eval(cnf,vs) == cnf_eval(other, vs)
+}
+
+
+function cnf_remove_tautologies(cnf: CNF) : (out: CNF)
+    ensures cnf_equivalent(cnf, out)
+{
+    set c | c in cnf && !clause_is_tautology(c)
+}
